More progress on open program semantics preservation

sepcomp/open_safety_preservation.v
@@ -9,19 +9,131 @@ Require Import compcert.common.AST.
 Require Import compcert.common.Globalenvs.
 
 Require Import msl.Axioms.
-Require Import sepcomp.extspec.
 Require Import sepcomp.mem_lemmas. (*needed for definition of mem_forward etc*)
-Require Import sepcomp.step_lemmas.
 Require Import sepcomp.core_semantics.
 Require Import sepcomp.effect_semantics.
-Require Import sepcomp.effect_simulations.
+Require Import sepcomp.trace_semantics.
 Require Import sepcomp.StructuredInjections.
+Require Import sepcomp.effect_simulations.
+Require Import sepcomp.effect_properties.
+Require Import sepcomp.extspec.
 
 Import SM_simulation.
 
 (** * Safety and semantics preservation *)
 
-Section safety_preservation_lemmas.
+Section safety.
+Context { G C D : Type }
+        (Hcore : CoopCoreSem G C)
+        (ge : G).
+
+Fixpoint safeN (n:nat) (c:C) (m:mem) : Prop :=
+  match n with
+    | O => True
+    | S n' => 
+      match halted Hcore c with
+        | None => 
+          exists c', exists m',
+            corestep Hcore ge c m c' m' /\
+            safeN n' c' m'
+        | Some i => True
+      end
+  end.
+
+Definition corestep_fun  :=
+  forall ge m q m1 q1 m2 q2 ,
+    corestep Hcore ge q m q1 m1 -> 
+    corestep Hcore ge q m q2 m2 -> 
+    (q1, m1) = (q2, m2).
+
+Lemma safe_downward1 :
+  forall n c m,
+    safeN (S n) c m -> safeN n c m.
+Proof.
+  induction n; simpl; intros; auto.
+  destruct (halted Hcore c); auto.
+  destruct H as [c' [m' [? ?]]].
+  exists c', m'; split; auto.
+Qed.
+
+Lemma safe_downward : 
+  forall (n n' : nat) c m,
+    le n' n ->
+    safeN n c m -> safeN n' c m.
+Proof.
+  do 6 intro. revert c m H0. induction H; auto.
+  intros. apply IHle. apply safe_downward1. auto.
+Qed.
+
+Lemma safe_corestep_forward:
+  corestep_fun -> 
+  forall c m c' m' n,
+    corestep Hcore ge c m c' m' -> safeN (S n) c m -> safeN n c' m'.
+Proof.
+  simpl; intros.
+  erewrite corestep_not_halted in H1; eauto.
+  destruct H1 as [c'' [m'' [? ?]]].
+  assert ((c',m') = (c'',m'')).
+  eapply H; eauto.
+  inv H3; auto.
+Qed.
+
+Lemma safe_corestepN_forward:
+  corestep_fun -> 
+  forall c m c' m' n n0,
+    corestepN Hcore ge n0 c m c' m' -> safeN (n + S n0) c m -> safeN n c' m'.
+Proof.
+  intros.
+  revert c m c' m' n H0 H1.
+  induction n0; intros; auto.
+  simpl in H0; inv H0.
+  eapply safe_downward in H1; eauto. omega.
+  simpl in H0. destruct H0 as [c2 [m2 [STEP STEPN]]].
+  apply (IHn0 _ _ _ _ n STEPN). 
+  assert (Heq: (n + S (S n0) = S (n + S n0))%nat) by omega.
+  rewrite Heq in H1.
+  eapply safe_corestep_forward in H1; eauto.
+Qed.
+
+Lemma safe_corestep_backward:
+  forall c m c' m' n,
+    corestep Hcore ge c m c' m' -> safeN (n - 1) c' m' -> safeN n c m.
+Proof.
+  simpl; intros.
+  induction n; simpl; auto.
+  erewrite corestep_not_halted; eauto.
+  exists c', m'; split; auto.
+  assert (Heq: (n = S n - 1)%nat) by omega.
+  rewrite Heq; auto.
+Qed.
+
+Lemma safe_corestepN_backward:
+  forall c m c' m' n n0,
+    corestepN Hcore ge n0 c m c' m' -> safeN (n - n0) c' m' -> safeN n c m.
+Proof.
+  simpl; intros.
+  revert c m c' m' n H H0.
+  induction n0; intros; auto.
+  simpl in H; inv H.
+  solve[assert (Heq: (n = n - 0)%nat) by omega; rewrite Heq; auto].
+  simpl in H. destruct H as [c2 [m2 [STEP STEPN]]].
+  assert (H: safeN (n - 1 - n0) c' m'). 
+  eapply safe_downward in H0; eauto. omega.
+  specialize (IHn0 _ _ _ _ (n - 1)%nat STEPN H). 
+  eapply safe_corestep_backward; eauto.
+Qed.
+
+End safety.
+
+Definition target_accessible mu m tm args b ofs :=
+  Mem.valid_block tm b /\ 
+  (locBlocksTgt mu b=false -> 
+    exists b0 d, 
+      foreign_of mu b0 = Some (b, d) 
+      /\ REACH m (getBlocks args) b0=true 
+      /\ Mem.perm m b0 (ofs-d) Max Nonempty).
+
+Section semantics_preservation.
 Context  {F V TF TV C D Z : Type}
          {source : @EffectSem (Genv.t F V) C}
          {target : @EffectSem (Genv.t TF TV) D}
@@ -29,485 +141,415 @@ Context  {F V TF TV C D Z : Type}
          {geT : Genv.t TF TV}
          {entry_points : list (val*val*signature)}
 
-  (sim : SM_simulation_inject source target geS geT entry_points)
-  (z : Z)
-  (c : C)
-  (d : D)
-  (m : mem)
-  (tm: mem)
+  (z_init : Z)
 
   (spec : ext_spec Z)
   (spec_closed : injection_closed spec)
+  (spec_ok : 
+    forall ef x tys args targs m rty rv m' tm z z' j,
+    ext_spec_pre spec ef x tys args z m -> 
+    ext_spec_post spec ef x rty rv z' m' -> 
+    Mem.inject (as_inj j) m tm -> 
+    val_list_inject (restrict (as_inj j) (vis j)) args targs -> 
+    mem_forward m m' -> 
+    Mem.unchanged_on (fun b ofs => REACH m (getBlocks args) b=false) m m'  -> 
+    exists j' rv' tm',
+      inject_incr (as_inj j) (as_inj j') 
+      /\ oval_inject (as_inj j') rv rv'
+      /\ Mem.inject (as_inj j') m' tm'
+      /\ sm_inject_separated j j' m tm 
+      /\ SM_wd j'
+      /\ sm_valid j' m' tm'
+      /\ mem_forward tm tm'
+      /\ Mem.unchanged_on (fun b ofs => 
+           ~target_accessible j m tm args b ofs) tm tm').
 
-  (SRC_DET : corestep_fun source)
+Section match_event.
 
-  (TGT_DET : corestep_fun target)
-  
-  (source_safe : forall n, safeN source spec geS n z c m)
-.
+Import Event.
+
+Inductive match_event : Event.t -> Event.t -> Prop :=
+| mk_match_event : 
+  forall j j' ev1 ev2,
+  Mem.inject (as_inj j) ev1.(pre_mem) ev2.(pre_mem) -> 
+  Mem.inject (as_inj j') ev1.(post_mem) ev2.(post_mem) -> 
+  Forall2 (val_inject (restrict (as_inj j) (vis j))) ev1.(args) ev2.(args) -> 
+  oval_inject (as_inj j') ev1.(rv) ev2.(rv) ->
+  match_event ev1 ev2.
+
+End match_event.
+
+Inductive match_trace : list Event.t -> list Event.t -> Prop :=
+| match_trace_nil : match_trace nil nil
+| match_trace_cons : 
+  forall tr1 tr2 ev1 ev2,
+  match_event ev1 ev2 -> 
+  match_trace tr1 tr2 -> 
+  match_trace (ev1 :: tr1) (ev2 :: tr2).
+
+Variable sim : SM_simulation_inject source target geS geT entry_points.
 
 Notation data := (sim.(SM_simulation.core_data _ _ _ _ _)).
 Notation ord  := (sim.(SM_simulation.core_ord _ _ _ _ _)).
 Notation match_state := (sim.(SM_simulation.match_state _ _ _ _ _)).
 
-Definition my_P := fun (x: data) => 
-  forall (j : SM_Injection) (z : Z) (c : C) (d : D) (m tm : mem),
-  (forall n : nat, safeN source spec geS n z c m) ->
-  match_state x j c m d tm ->
-  (exists ef sig vals, at_external source c = Some (ef, sig, vals))
-   \/ ((exists rv, halted source c = Some rv) \/
-       (exists cd' j' c' m',
-         corestep_plus source geS c m c' m'
-         /\ ((exists d' tm', corestep_plus target geT d tm d' tm'
-              /\ match_state cd' j' c' m' d' tm')
-         \/ (exists rv, halted source c' = Some rv 
-              /\ match_state cd' j' c' m' d tm)
-         \/ (exists ef sig vals, 
-               at_external source c' = Some (ef, sig, vals)
-              /\ match_state cd' j' c' m' d tm)))).
-
-Lemma corestep_ord:
-  forall cd j,
+Inductive trace_match_state : 
+  data -> SM_Injection -> Z*list Event.t*C -> mem -> Z*list Event.t*D -> mem -> Prop :=
+| mk_trace_match_state :
+  forall j tr z c m ttr d tm cd,
+  match_trace tr ttr -> 
   match_state cd j c m d tm -> 
-  (exists ef sig vals, at_external source c = Some (ef, sig, vals))
-   \/ (exists rv, halted source c = Some rv) 
-   \/ (exists cd' j' c' m',
-         corestep_plus source geS c m c' m'
-         /\ ((exists d' tm', corestep_plus target geT d tm d' tm'
-                          /\ match_state cd' j' c' m' d' tm')
-          \/ (exists rv, halted source c' = Some rv 
-                          /\ match_state cd' j' c' m' d tm)
-          \/ (exists ef sig vals, 
-                at_external source c' = Some (ef, sig, vals)
-                          /\ match_state cd' j' c' m' d tm))).
-Proof.
-assert (my_well_founded_induction
-     : (forall x, (forall y, ord y x -> my_P y) -> my_P x) ->
-       forall a, my_P a).
-  solve[apply well_founded_induction; destruct sim; auto].
-unfold my_P in my_well_founded_induction.
-destruct sim; simpl in *.
-intros cd j H; simpl.
-clear match_validblocks0 core_halted0 
-  core_initial0 core_at_external0 eff_after_external0.
-revert j z c d m tm source_safe H.
-apply my_well_founded_induction; auto.
-intros.
-case_eq (at_external source c).
-{ intros [[ef sig] args] AT_EXT.
-  left; exists ef, sig, args; auto. }
-intros AT_EXT.
-case_eq (halted source c).
-intros.
-solve[right; left; exists v; auto].
-intros HALTED_NONE.
-generalize H0 as SAFE; intro.
-specialize (H0 (S O)); simpl in H0.
-rewrite HALTED_NONE in H0.
-case_eq (at_external source c).
-intros [[ef sig] args] AT_EXT'.
-rewrite AT_EXT' in AT_EXT; congruence.
-intros AT_EXT'; rewrite AT_EXT' in H0.
-destruct H0 as [c2 [m2 [STEP _]]].
-generalize STEP as STEP'; intro.
-eapply core_diagram0 in STEP; eauto.
-clear AT_EXT.
-destruct STEP as [d2 [tm2 [cd2 [j2 [? [? [? [? [? [? H2]]]]]]]]]].
-destruct H2.
-right; right.
-exists cd2, j2, c2, m2.
-split; auto.
-solve[exists O; simpl; exists c2, m2; split; auto].
-solve[left; exists d2, tm2; split; auto].
-destruct H2 as [H2 ORD].
-specialize (H _ ORD j2 z c2 d2 m2 tm2).
-assert (SAFE': forall n, safeN source spec geS n z c2 m2).
-  solve[intros n; eapply safe_corestep_forward; eauto].
-specialize (H SAFE' H5).
-destruct H2 as [n H2].
-destruct n. inv H2.
-destruct H.
-destruct H as [ef [sig [args AT_EXT]]].
-right; right.
-exists cd2, j2, c2, m2.
-split; auto.
-solve[exists O; simpl; exists c2, m2; split; auto].
-solve[right; right; exists ef, sig, args; auto].
-destruct H.
-destruct H as [rv HALTED].
-right; right.
-exists cd2, j2, c2, m2.
-split; auto.
-solve[exists O; simpl; exists c2, m2; split; auto].
-solve[right; left; exists rv; split; auto].
-destruct H as [cd' [j' [c' [m' [STEPN H]]]]].
-destruct H as [H|[H|H]].
-destruct H as [d' [tm' [TSTEP' MATCH']]].
-right; right.
-exists cd', j', c', m'.
-split; auto. 
-destruct STEPN as [n STEPN].
-exists (S n).
-simpl.
-exists c2, m2.
-split; auto.
-solve[left; exists d', tm'; split; auto].
-destruct H as [rv [HALT MATCH']].
-right; right.
-exists cd', j', c', m'.
-split; auto. 
-destruct STEPN as [n STEPN].
-exists (S n).
-simpl.
-exists c2, m2.
-split; auto.
-solve[right; left; exists rv; split; auto].
-destruct H as [ef [sig [args AT_EXT]]].
-right; right.
-exists cd', j', c', m'.
-split; auto. 
-destruct STEPN as [n STEPN].
-exists (S n).
-simpl.
-exists c2, m2.
-split; auto.
-solve[right; right; exists ef, sig, args; auto].
-right; right.
-exists cd2, j2, c2, m2.
-split; auto. 
-solve[exists O; simpl; exists c2, m2; split; auto].
-left. 
-exists d2, tm2.
-split; auto.
-exists n; auto.
-Qed.
+  trace_match_state cd j (z,tr,c) m (z,ttr,d) tm. 
 
-Notation EXIT z rv m := (ext_spec_exit spec (Some rv) z m).
-Notation P ef x tys vals z m  := (ext_spec_pre spec ef x tys vals z m).
+Variables 
+(SRC_DET : corestep_fun source)
+(TGT_DET : corestep_fun target).
 
-Definition halt_match z c m d tm := 
-  exists rv trv, 
-    halted source c = Some rv 
-    /\ halted target d = Some trv
-    /\ EXIT z rv m 
-    /\ EXIT z trv tm.
+Notation tr_source := (TraceSemantics.coopsem z_init source spec).
+Notation tr_target := (TraceSemantics.coopsem z_init target spec).
 
-Definition at_external_match z c m d tm :=
-  exists ef sig x tys vals tvals,
-    at_external source c = Some (ef, sig, vals) 
-    /\ at_external target d = Some (ef, sig, tvals)
-    /\ P ef x tys vals z m
-    /\ P ef x tys tvals z tm.
-
-Lemma corestep_ord':
-  forall cd j,
+Lemma corestep_plus_match {c m d tm c' m' cd j} :
+  corestep_plus source geS c m c' m' -> 
   match_state cd j c m d tm -> 
-  at_external_match z c m d tm
-  \/ halt_match z c m d tm 
-  \/ (exists cd' j' c' m', 
-         corestep_plus source geS c m c' m' /\ 
-               ((match_state cd' j' c' m' d tm /\ at_external_match z c' m' d tm)
-            \/ ((match_state cd' j' c' m' d tm /\ halt_match z c' m' d tm)
-            \/ (exists d' tm', 
-                  corestep_plus target geT d tm d' tm'
-                  /\ match_state cd' j' c' m' d' tm')))).
+  exists d' tm' cd' j', 
+    corestep_plus target geT d tm d' tm'
+    /\ match_state cd' j' c' m' d' tm'.
+Admitted.
+
+Lemma REACH_mono':
+  forall B1 B2 : block -> bool,
+  (forall b : block, B1 b = true -> B2 b = true) ->
+  forall (m : mem) (b : block), REACH m B2 b = false -> REACH m B1 b = false.
 Proof.
-intros.
-generalize H as MATCH; intro.
-apply corestep_ord in H.
-destruct H.
-{
-destruct H as [ef [sig [args AT_EXT]]].
-left.
-unfold at_external_match.
-destruct sim; simpl in *.
-clear match_validblocks0 core_diagram0 
-  core_initial0 core_halted0 eff_after_external0.
-generalize AT_EXT as AT_EXT'; intro.
-apply (core_at_external0 cd j c m d tm) in AT_EXT; auto.
-destruct AT_EXT as [INJ [targs [VINJ TAT_EXT]]].
-exists ef, sig.
-generalize (source_safe (S O)); simpl.
-rewrite AT_EXT'.
-assert (halted source c = None) as ->.
-  solve[destruct (at_external_halted_excl source c); try congruence; auto].
-intros [x [HP ?]].
-exists x, (sig_args sig), args, targs; split; auto.
-split; auto.
-split; auto.
-eapply (P_closed spec_closed); eauto.
-apply forall_vals_inject_restrictD in VINJ.
-solve[apply forall_inject_val_list_inject; auto].
-}
-destruct H.
-{
-destruct H as [rv HALT].
-right; left.
-unfold halt_match.
-destruct sim; simpl in *.
-clear match_validblocks0 core_diagram0 
-  core_initial0 core_at_external0 eff_after_external0.
-generalize HALT as HALT'; intro.
-apply (core_halted0 cd j c m d tm) in HALT; auto.
-destruct HALT as [rv' [INJ [HALT INJ2]]].
-exists rv, rv'.
-split; auto.
-split; auto.
-generalize (source_safe (S O)); simpl; rewrite HALT'.
-assert (at_external source c = None) as ->.
-  solve[destruct (at_external_halted_excl source c); try congruence; auto].
-intros; split; auto.
-eapply (exit_closed spec_closed); eauto.
-apply inject_restrict; auto.
-solve[destruct sim; eapply match_visible0; eauto].
-}
-{
-destruct H as [cd' [j' [c' [m' [STEPN ?]]]]].
-destruct H as [H|H].
-destruct H as [d' [tm' [TSTEPN MATCH']]].
-right; right.
-exists cd', j', c', m'.
-split; auto.
-right; right.
-exists d', tm'.
-solve[split; auto].
-destruct H.
-destruct H as [rv [HALT MATCH']].
-right; right.
-exists cd', j', c', m'.
-split; auto.
-right.
-left.
-split; auto.
-unfold halt_match.
-destruct sim; simpl in *.
-clear match_validblocks0 core_diagram0 
-  core_initial0 core_at_external0 eff_after_external0.
-generalize HALT as HALT'; intro.
-apply (core_halted0 cd' j' c' m' d tm) in HALT; auto.
-destruct HALT as [rv' [INJ [HALT INJ2]]].
-exists rv, rv'.
-split; auto.
-split; auto.
-assert (H: forall n, safeN source spec geS n z c' m').
-  intro n. 
-  destruct STEPN as [n0 STEPN].
-  specialize (source_safe (n + S (S n0))). 
-  solve[eapply safe_corestepN_forward in source_safe; eauto].
-generalize (H (S O)); simpl; rewrite HALT'.
-assert (at_external source c' = None) as ->.
-   solve[destruct (at_external_halted_excl source c'); try congruence; auto].
-intros; split; auto.
-eapply (exit_closed spec_closed); eauto.
-apply inject_restrict; auto.
-solve[destruct sim; eapply match_visible0; eauto].
-destruct H as [ef [sig [args [AT_EXT MATCH']]]].
-right; right.
-exists cd', j', c', m'.
-split; auto.
-left.
-split; auto.
-unfold at_external_match.
-destruct sim; simpl in *.
-clear match_validblocks0 core_diagram0 
-  core_initial0 core_halted0 eff_after_external0.
-generalize AT_EXT as AT_EXT'.
-apply (core_at_external0 cd' j' c' m' d tm) in AT_EXT; auto.
-destruct AT_EXT as [INJ [targs [VINJ TAT_EXT]]].
-intros AT_EXT'.
-exists ef, sig.
-assert (H: forall n, safeN source spec geS n z c' m').
-  intro n. 
-  destruct STEPN as [n0 STEPN].
-  specialize (source_safe (n + S (S n0))). 
-  solve[eapply safe_corestepN_forward in source_safe; eauto].
-generalize (H (S O)); simpl; rewrite AT_EXT'.
-assert (halted source c' = None) as ->.
-   solve[destruct (at_external_halted_excl source c'); try congruence; auto].
-intros [x]; intros [HP]; intros H2.
-exists x, (sig_args sig), args, targs; split; auto.
-split; auto.
-split; auto.
-eapply (P_closed spec_closed); eauto.
-apply forall_vals_inject_restrictD in VINJ.
-solve[apply forall_inject_val_list_inject; auto].
-}
+intros ? ? SUB m b HR.
+case_eq (REACH m B1 b); auto.
+solve[intros H; generalize (REACH_mono _ _ SUB _ _ H); congruence].
 Qed.
 
-End safety_preservation_lemmas.
+Lemma REACH_as_inj': forall mu (WD: SM_wd mu) m1 m2 vals1 vals2 
+        (MemInjMu : Mem.inject (as_inj mu) m1 m2)
+        (ValInjMu : Forall2 (val_inject (as_inj mu)) vals1 vals2) b1
+        (R : REACH m1 (getBlocks vals1) b1 = true)
+        B (HB: forall b b2 d, shared_of mu b = Some(b2,d) -> B b2 = true),
+      exists b2 d, as_inj mu b1 = Some (b2, d) /\ 
+                   REACH m2 (fun b => orb (getBlocks vals2 b) (B b)) b2 = true.
+Proof. intros.
+ eapply (REACH_inject _ _ _ MemInjMu); try eassumption.
+ clear R. simpl; intros.
+ destruct (getBlocks_inject _ _ _ ValInjMu _ H) as [b2 [d [J G]]].
+ exists b2, d. rewrite J, G. intuition.
+Qed.
 
-(** ** Termination preservation *)
+Lemma REACH_as_inj_REACH': forall mu (WD: SM_wd mu) m1 m2 vals1 vals2 
+        (MemInjMu : Mem.inject (as_inj mu) m1 m2)
+        (ValInjMu : Forall2 (val_inject (as_inj mu)) vals1 vals2) b1
+        (R : REACH m1 (getBlocks vals1) b1 = true),
+      exists b2 d, as_inj mu b1 = Some (b2, d) /\ 
+                   REACH m2 (getBlocks vals2) b2 = true.
+Proof. intros.
+  destruct (REACH_as_inj' _ WD _ _ _ _ MemInjMu ValInjMu _ R (fun b => true))
+       as [b2 [d [ASI _]]]. trivial.
+  exists b2, d. split; trivial.
+  destruct (REACH_inject _ _ _ MemInjMu) 
+    with (B1 := getBlocks vals1) (B2 := getBlocks vals2) (b1 := b1); auto.
+  intros.
+  solve[apply getBlocks_inject with (vals1 := vals1); auto]. 
+  destruct H as [bb2 [ASI' RR]]; rewrite ASI' in ASI; inv ASI.
+  assumption.
+Qed.
 
-Section termination_preservation.
-Context  {F V TF TV C D Z data : Type}
-         {source : @EffectSem (Genv.t F V) C}
-         {target : @EffectSem (Genv.t TF TV) D}
-         {geS : Genv.t F V}
-         {geT : (Genv.t TF TV)}
-         {entry_points : list (val*val*signature)}
+Definition visSrc mu b := locBlocksSrc mu b || frgnBlocksSrc mu b.
 
-  (sim : SM_simulation_inject source target geS geT entry_points)
-  (z : Z)
-  (c : C)
-  (d : D)
-  (m : mem)
-  (tm: mem)
+Definition visTgt mu b := locBlocksTgt mu b || frgnBlocksTgt mu b.
 
-  (spec : ext_spec Z)
-  (spec_closed : injection_closed spec)
+Definition marshal j m args tm targs := 
+  Build_SM_Injection
+  (fun _ => false) (fun _ => false) 
+  (fun _ => false) (fun _ => false) 
+  (fun _ => None)
+  (REACH m (getBlocks args))
+  (REACH tm (getBlocks targs))
+  (REACH m (getBlocks args))
+  (REACH tm (getBlocks targs))
+  j.
 
-  (SRC_DET : corestep_fun source)
+Lemma as_inj_marshal j m args tm targs :
+  as_inj (marshal j m args tm targs) = j.
+Proof. 
+unfold marshal, as_inj, join; simpl.
+extensionality b.
+destruct (j b); auto.
+destruct p; auto.
+Qed.
 
-  (TGT_DET : corestep_fun target)
+Lemma foreign_of_marshal j m args tm targs :
+  foreign_of (marshal j m args tm targs) 
+  = restrict j (REACH m (getBlocks args)).
+Proof. 
+unfold marshal, as_inj, join, restrict; simpl.
+extensionality b.
+destruct (j b); auto.
+Qed.
 
-  (source_safe : forall n, safeN source spec geS n z c m)
-.
+Lemma locBlocksTgt_marshal j m args tm targs :
+  locBlocksTgt (marshal j m args tm targs) = (fun _ => false).
+Proof. unfold marshal, as_inj, join, restrict; auto. Qed.
 
-Notation data := (sim.(SM_simulation.core_data _ _ _ _ _)).
-Notation ord  := (sim.(SM_simulation.core_ord _ _ _ _ _)).
-Notation match_state := (sim.(SM_simulation.match_state _ _ _ _ _)).
+Lemma vis_marshal j m args tm targs :
+  vis (marshal j m args tm targs) = REACH m (getBlocks args).
+Proof. unfold marshal, vis; simpl; auto. Qed.
 
-Lemma termination_preservation:
-  forall cd j c' m' rv1,
+Lemma yielded_source_yielded_target {cd j c d m tm} :
   match_state cd j c m d tm -> 
-  corestep_star source geS c m c' m' -> 
-  halted source c' = Some rv1 -> 
-  exists d' tm' rv2, 
-     corestep_star target geT d tm d' tm' 
-  /\ halted target d' = Some rv2.
+  TraceSemantics.yielded source c -> 
+  TraceSemantics.yielded target d.
+Admitted.
+
+Lemma semantics_preservation_aux {n c c' d m m' tm cd j} : 
+  trace_match_state cd j c m d tm -> 
+  corestepN tr_source geS n c m c' m' -> 
+  exists cd' j' d' tm',
+    corestepN tr_target geT n d tm d' tm' 
+    /\ trace_match_state cd' j' c' m' d' tm'.
 Proof.
-intros.
-destruct H0 as [n H0].
-revert cd j c m d tm H H0 source_safe.
-induction n; intros.
-simpl in H0. symmetry in H0; inv H0.
-apply (corestep_ord' sim z c d m tm spec) in H; auto.
-destruct H.
-destruct H as [ef [sig [x [tys [args [targs [A [B [X Y]]]]]]]]].
-elimtype False.
-solve[destruct (at_external_halted_excl source c); try congruence; auto].
-cut (@halt_match F V _ _ C D Z source target spec z c m d tm). intro.
-unfold halt_match in H0.
-destruct H0 as [rv [trv [? [? [? ?]]]]].
-exists d, tm, trv.
-split; auto.
-solve[exists O; simpl; auto].
-destruct H; auto.
-destruct H as [? [? [? [? [STEP ?]]]]].
-destruct STEP as [n STEP].
-simpl in STEP.
-destruct STEP as [c2 [m2 [STEP ?]]].
-apply corestep_not_halted in STEP.
-rewrite STEP in H1; congruence.
-simpl in H0.
-destruct H0 as [c2 [m2 [? ?]]].
-destruct sim; simpl in *.
-clear match_validblocks0 core_halted0 
-  core_initial0 core_at_external0 eff_after_external0.
-generalize H0 as H0'; intro.
-eapply core_diagram0 in H0; eauto.
-destruct H0 as [d2 [tm2 [cd2 [j2 [? [? [? [? [? [? ?]]]]]]]]]].
-assert (SAFE: forall n, safeN source spec geS n z c2 m2). 
-  intros n0.
-  solve[eapply safe_corestep_forward in H0'; eauto].
-specialize (IHn cd2 j2 c2 m2 d2 tm2 H5 H2 SAFE).
-destruct IHn as [d' [tm' [trv [? ?]]]].
-exists d', tm', trv.
-split; auto.
-eapply corestep_star_trans; eauto.
-destruct H8.
-destruct H8 as [n0 H8].
-solve[exists (S n0); auto].
-destruct H8; auto.
+intros TRMATCH STEPN; revert cd j c m d tm TRMATCH STEPN.
+induction n; simpl; intros cd j c m d tm TRMATCH STEPN.
+solve[inv STEPN; exists cd, j, d, tm; split; auto].
+destruct STEPN as [[[z2 tr] c2] [m2 [STEP STEPN]]].
+destruct c as [[z tr2] c].
+destruct d as [[tz ttr] d].
+assert (MATCH: match_state cd j c m d tm). 
+  solve[inv TRMATCH; auto].
+inv STEP; rename H8 into STEPP.
+{ (*internal step case*)
+generalize (corestep_plus_match STEPP MATCH).
+intros [d2 [tm2 [cd2 [j2 [STEPP' MATCH2]]]]].
+assert (TRMATCH2: trace_match_state cd2 j2 (z2,tr,c2) m2 (z2,ttr,d2) tm2).
+  constructor; auto.
+  solve[inv TRMATCH; auto].
+generalize (IHn _ _ _ _ _ _ TRMATCH2 STEPN).
+intros [cd' [j' [d' [tm' [TSTEPN' TRMATCH']]]]].
+exists cd', j', d', tm'; split; auto.
+exists (tz,ttr,d2), tm2; split; auto.
+constructor; auto.
+solve[eapply yielded_source_yielded_target in H9; eauto].
+assert (tz = z2) as -> by (inv TRMATCH; auto). 
+solve[auto].
+}
+Arguments core_at_external : default implicits.
+{ (*external step case*)
+assert (exists targs, 
+  at_external target d = Some (ef, sig, targs)
+  /\ val_list_inject (restrict (as_inj j) (vis j)) args targs) 
+  as [targs [AT VALINJ]].
+  inv TRMATCH; eapply core_at_external in H15; eauto.
+  destruct H15 as [_ [targs [? ?]]]; exists targs; split; auto.
+  solve[apply forall_inject_val_list_inject; auto].
+assert (INJ: Mem.inject (as_inj j) m tm). 
+  inv TRMATCH; eapply core_at_external in H15; eauto.
+  solve[destruct H15 as [? _]; auto].
+set (pubSrc' := fun b => andb (locBlocksSrc j b) (REACH m (exportedSrc j args) b)).
+set (pubTgt' := fun b => andb (locBlocksTgt j b) (REACH tm (exportedTgt j targs) b)).
+set (nu := replace_locals j pubSrc' pubTgt').
+
+set (mu := marshal (as_inj j) m args tm targs).
+assert (MU_INJ: Mem.inject (as_inj mu) m tm). 
+  solve[unfold mu; rewrite as_inj_marshal; auto].
+assert (MU_VALINJ: val_list_inject (restrict (as_inj mu) (vis mu)) args targs).
+  inv TRMATCH; eapply core_at_external in H15; eauto.
+  destruct H15 as [_ [? [VALINJ' ATEXT]]].
+  rewrite ATEXT in AT; inv AT.
+  unfold mu; rewrite as_inj_marshal, vis_marshal.
+  apply forall_inject_val_list_inject.
+  admit.
+
+generalize (spec_ok ef x (sig_args sig) args targs m 
+  (sig_res sig) (Some rv) m2 tm _ _ mu H11 H12 MU_INJ MU_VALINJ H10 STEPP).
+intros [mu2 [trv [tm2 [INCR [RVALINJ [INJ2 [SEP2 [WD2 [VAL2 [TFWD2 TUNCH]]]]]]]]]].
+
+set (nu2 := reestablish nu mu2).
+set (frgnSrc' := fun b : block =>
+     DomSrc nu2 b &&
+     (negb (locBlocksSrc nu2 b) && REACH m2 (exportedSrc nu2 (rv :: nil)) b)).
+
+assert (exists trv0, trv = Some trv0) as [trv0 ->]. 
+  simpl in RVALINJ; destruct trv as [trv|]; try solve[elimtype False; auto].
+  solve[exists trv; auto].
+
+set (frgnTgt' := fun b : block =>
+     DomTgt nu2 b &&
+     (negb (locBlocksTgt nu2 b) &&
+      REACH tm2 (exportedTgt nu2 (trv0 :: nil)) b)).
+
+set (nu' := replace_externs nu2 frgnSrc' frgnTgt').
+
+(* admits here mostly related to reestablish -- *)
+assert (VALINJ': Forall2 (val_inject (as_inj j)) args targs). 
+  admit.
+assert (VALINJ'': Forall2 (val_inject (restrict (as_inj j) (vis j))) args targs).
+  solve[apply val_list_inject_forall_inject; auto].
+
+assert (EINCR: extern_incr nu nu2). 
+  apply reestablish_extern_incr'; auto.
+  admit. 
+  unfold nu; rewrite replace_locals_as_inj.
+  apply inject_incr_trans with (f2 := as_inj mu); auto.
+  unfold mu; rewrite as_inj_marshal.
+  apply inject_incr_refl.
+  admit.
+  admit.
+assert (NU_SEP: sm_inject_separated nu nu2 m tm). 
+  admit.
+assert (NU_WD: SM_wd nu2).
+  apply reestablish_wd'; auto.
+  admit.
+  unfold nu; rewrite replace_locals_as_inj.
+  apply inject_incr_trans with (f2 := as_inj mu); auto.
+  unfold mu; rewrite as_inj_marshal.
+  apply inject_incr_refl.
+  intros ? ? ? AS.
+  unfold nu. 
+  rewrite replace_locals_locBlocksSrc, replace_locals_locBlocksTgt.
+  rewrite replace_locals_extBlocksSrc, replace_locals_extBlocksTgt.
+  split; auto.
+  admit. (*by j WD*)
+  admit. (*by j WD*)
+  admit.
+assert (NU_VAL: sm_valid nu2 m2 tm2). admit.
+assert (NU_INJ: Mem.inject (as_inj nu2) m2 tm2). admit.
+assert (NU_VINJ: val_inject (as_inj nu2) rv trv0). admit.
+
+generalize (@eff_after_external _ _ _ _ _ _ _ _ _ _ _ 
+  sim cd j c d m ef args tm sig targs ef sig INJ MATCH H6 AT VALINJ''
+  pubSrc' refl_equal
+  pubTgt' refl_equal
+  nu refl_equal nu2 rv m2 trv0 tm2 
+  EINCR NU_SEP NU_WD NU_VAL NU_INJ NU_VINJ H10 TFWD2
+  frgnSrc' refl_equal
+  frgnTgt' refl_equal
+  nu' refl_equal).
+
+destruct 1 as [acd [ac [ad [AFT1 [AFT2 AMATCH]]]]]; auto. 
+apply unch_on_validblock with (V := 
+  fun b ofs => REACH m (getBlocks args) b=false); auto.
+intros b ofs BVAL [X Y].
+unfold nu in Y; unfold pubSrc', pubTgt' in Y. 
+rewrite replace_locals_pubBlocksSrc in Y. 
+unfold nu in X; rewrite replace_locals_locBlocksSrc in X.
+rewrite X in Y; simpl in Y.
+apply REACH_mono' with (B2 := exportedSrc j args); auto.
+solve[intros b'; unfold exportedSrc; intros ->; auto].
+
+apply unch_on_validblock with (V := 
+  fun b ofs => ~target_accessible mu m tm args b ofs); auto.
+intros b ofs BVAL [X Y].
+unfold nu in Y; unfold pubSrc', pubTgt' in Y. 
+rewrite replace_locals_pubBlocksSrc in Y.
+rewrite replace_locals_local in Y.
+unfold nu in X; rewrite replace_locals_locBlocksTgt in X.
+unfold target_accessible; unfold mu; simpl; intros [VAL TA].
+destruct TA as [b0 [d0 [INJ0 [HR' PERM]]]]; auto.
+assert (HR'': REACH m (exportedSrc j args) b0=true).
+  apply REACH_mono with (B1 := getBlocks args); auto.
+  solve[unfold exportedSrc; intros ? ->; auto].
+Arguments match_sm_wd : default implicits.
+generalize (match_sm_wd sim _ _ _ _ _ _ MATCH); intros WD.
+apply REACH_as_inj_REACH with (m2 := tm) (vals2 := targs) in HR''; auto.
+destruct HR'' as [b' [d' [INJ'' HR'']]].
+assert (b = b' /\ d0 = d') as [? ?]. 
+  unfold mu in INJ0; rewrite HR' in INJ0.
+  solve[rewrite INJ0 in INJ''; inv INJ''; auto].
+subst b' d'.
+
+assert (local_of j b0 = Some (b, d0) /\ locBlocksSrc j b0=true)
+  as [LOCOF LSRC].
+  generalize INJ''; clear INJ''.
+  unfold as_inj, join.
+  case_eq (extern_of j b0); auto.
+  intros [? ?] EXT; inversion 1; subst.
+  apply extern_DomRng' in EXT; auto.
+  destruct EXT as [_ [_ [_ [TLOC _]]]].
+  solve[rewrite TLOC in X; congruence].
+  intros; split; auto.
+  apply local_DomRng in INJ''; auto.
+  destruct INJ''; auto.
+destruct (Y _ _ LOCOF).
+solve[apply H; apply PERM].
+assert (HR''': REACH m (exportedSrc j args) b0=true).
+  apply REACH_mono with (B1 := getBlocks args); auto.
+  solve[unfold exportedSrc; intros ? ->; auto].
+rewrite LSRC, HR''' in H; simpl in H; congruence.
+
+Arguments match_validblocks : default implicits.
+generalize (match_validblocks sim _ _ _ _ _ _ MATCH); intros ?.
+edestruct eff_after_check1 
+  with (mu := j) (m1 := m) (m2 := tm) (vals1 := args) (vals2 := targs)
+       (pubSrc' := pubSrc') (pubTgt' := pubTgt'); auto.
+solve[apply (match_sm_wd sim _ _ _ _ _ _ MATCH)].
+set (tr2' := Event.mk m m2 args (Some rv) :: tr2).
+set (ttr' := Event.mk tm tm2 targs (Some trv0) :: ttr).
+destruct (IHn acd nu' (z2,tr2',ac) m2 (z2,ttr',ad) tm2)
+  as [cd' [j' [d' [tm' [STEPN' MATCH']]]]].
+constructor. constructor. econstructor; eauto.
+solve[apply val_list_inject_forall_inject; auto].
+solve[inv TRMATCH; auto].
+solve[auto].
+solve[rewrite H13 in AFT1; inv AFT1; apply STEPN].
+
+exists cd', j', d', tm'; split; auto.
+exists (z2,ttr',ad), tm2; split; auto.
+econstructor; eauto. 
+
+apply unch_on_validblock with (V := 
+  fun b ofs => ~target_accessible mu m tm args b ofs); auto.
+intros b ofs X Y. 
+unfold target_accessible; intros [VAL TA]. 
+destruct TA as [b0 [d0 [FR [RC PERM]]]]; auto.
+apply REACH_as_inj_REACH' with (m2 := tm) (vals2 := targs) (mu := j) in RC; auto.
+destruct RC as [b2 [d2 [INJ' RR]]].
+assert (b = b2). 
+  apply foreign_in_all in FR. 
+  unfold mu in FR; rewrite as_inj_marshal in FR.
+  solve[rewrite FR in INJ'; inv INJ'; auto].
+solve[subst; congruence].
+solve[apply (match_sm_wd sim _ _ _ _ _ _ MATCH)].
+
+instantiate (1 := x).
+assert (VALINJ''' : val_list_inject (as_inj j) args targs). 
+  solve[apply forall_inject_val_list_inject; auto].
+generalize (P_closed spec_closed ef x (sig_args sig) z H11 VALINJ''' INJ).
+assert (z = tz) as -> by (inv TRMATCH; auto).
+solve[auto].
+generalize (Q_closed spec_closed ef x 
+  (sig_res sig) (Some rv) z2 (Some trv0) H12 RVALINJ INJ2).
+solve[auto]. }
 Qed.
 
-End termination_preservation.
+Lemma target_tracesem_det {x x' x'' m m' m'' n} :
+  corestepN tr_target geT n x m x' m' -> 
+  corestepN tr_target geT n x m x'' m'' -> 
+  x'=x'' /\ m'=m''.
+Admitted.
 
-Local Open Scope nat_scope.
-
-(** ** Safety & semantics preservation *)
-
-Section safety_preservation.
-Variables F V TF TV C D Z : Type.
-Variable source : @EffectSem (Genv.t F V) C.
-Variable target : @EffectSem (Genv.t TF TV) D.
-Variable geS : Genv.t F V.
-Variable geT : (Genv.t TF TV).
-Variable entry_points : list (val*val*signature).
-Variable (SRC_DET : corestep_fun source).
-Variable (TGT_DET : corestep_fun target).
-
-Lemma safety_preservation:
-  forall sim : SM_simulation_inject source target geS geT entry_points,
-    let data := (sim.(SM_simulation.core_data _ _ _ _ _)) in
-    let ord  := (sim.(SM_simulation.core_ord _ _ _ _ _)) in
-    let match_state := (sim.(SM_simulation.match_state _ _ _ _ _)) in
-      forall 
-        (c : C)
-        (d : D)
-        (m : mem)
-        (tm: mem)
-        (P : val -> mem -> Prop)
-        (P_good : forall j v tv m tm, 
-                    val_inject j v tv -> Mem.inject j m tm -> P v m -> P tv tm)
-        (MATCH : exists (cd: data) (j: SM_Injection), match_state cd j c m d tm)
-        (source_safe : forall n, safeN source geS P n c m),
-  forall n, safeN target geT P n d tm.
-Proof.
-intros until n.
-destruct MATCH as [cd [j MATCH2]].
-revert cd j c m d tm MATCH2 source_safe.
-induction n; simpl; auto.
-intros.
-apply (corestep_ord' sim c d m tm P) in MATCH2; auto.
-destruct MATCH2 as [H|H].
-destruct H as [rv [rv' [H1 [H2 [H3 H4]]]]].
-rewrite H2; auto.
-destruct H as [cd' [j' [c' [m' [STEPN [[H1 H2]|H]]]]]].
-destruct H2 as [rv [rv' [A1 [A2 [A3 A4]]]]].
-rewrite A2; auto.
-destruct H as [d' [tm' [TSTEPN MATCH']]].
-destruct TSTEPN as [n0 TSTEPN].
-cut (halted target d = None). intros ->.
-simpl in TSTEPN.
-destruct TSTEPN as [d2 [tm2 [TSTEP TSTEPN]]].
-exists d2, tm2.
-split; auto.
-cut (safeN target geT P (n - n0) d' tm'). intro SAFE.
-apply (@safe_corestepN_backward _ _ _ _ _ _ _ _ _ _ _ TSTEPN SAFE).
-cut (safeN target geT P n d' tm'). intro.
-apply safe_downward with (n' := (n - n0)%nat) in H.
-apply H. omega.
-apply (IHn _ _ _ _ _ _ MATCH').
-intros n1.
-destruct STEPN as [n2 STEPN].
-specialize (source_safe (n1 + S (S n2))).
-generalize @safe_corestepN_forward. intro FORW.
-solve[apply (FORW _ _ _ _ _ SRC_DET _ _ _ _ _ _ STEPN source_safe)].
-simpl in TSTEPN.
-destruct TSTEPN as [d2 [tm2 [STEP ?]]].
-solve[apply corestep_not_halted in STEP; auto].
+Lemma semantics_preservation z z' c c' d m m' tm tr cd j n :
+  match_state cd j c m d tm -> 
+  corestepN tr_source geS n (z,nil,c) m (z',tr,c') m' -> 
+  (exists z'' d' tm' ttr, corestepN tr_target geT n (z,nil,d) tm (z'',ttr,d') tm')
+  /\ forall z'' d' tm' ttr, 
+     corestepN tr_target geT n (z,nil,d) tm (z'',ttr,d') tm' -> 
+     match_trace tr ttr.
+Proof.  
+intros MATCH STEPN.
+assert (TRMATCH: trace_match_state cd j (z,nil,c) m (z,nil,d) tm).
+  constructor; auto.
+  solve[constructor; auto].
+generalize (semantics_preservation_aux TRMATCH STEPN).
+intros [cd' [j' [[[tz' ttr] d'] [tm' [TSTEPN TTRMATCH]]]]].
+split; [solve[exists tz', d', tm', ttr; auto]|].
+intros tz'' d'' tm'' ttr' TSTEPN'.
+generalize (target_tracesem_det TSTEPN TSTEPN'); intros [X Y].
+inv X.
+solve[inv TTRMATCH; auto].
 Qed.
 
-Lemma halted_safe: 
-  forall c m c' m' (P: val -> mem -> Prop) rv, 
-  corestep_star source geS c m c' m' -> 
-  halted source c' = Some rv -> 
-  P rv m' -> 
-  (forall n, safeN source geS P n c m).
-Proof.
-intros.
-destruct H as [n0 H].
-revert c m H H0.
-induction n0.
-simpl. intros. inv H.
-destruct n; simpl; auto.
-solve[rewrite H0; auto].
-simpl.
-intros c0 m0 [c2 [m2 [STEP STEPN]]] HALTED.
-apply (safe_corestep_backward _ _ _ _ _ _ _ _ STEP).
-generalize (IHn0 _ _ STEPN HALTED); intros SAFEN.
-solve[apply safe_downward with (n1 := n); auto; omega].
-Qed.
-
-End safety_preservation.
+End semantics_preservation.
