sepcomp/trace_semantics.v
@@ -10,7 +10,7 @@ Require Import compcert.common.Events.
 
 Require Import sepcomp.core_semantics.
 Require Import sepcomp.effect_semantics.
-Require Import sepcomp.effect_safety.
+Require Import sepcomp.effect_simulations.
 Require Import sepcomp.extspec.
 Require Import sepcomp.mem_lemmas.
 
@@ -30,43 +30,43 @@ End Event.
 
 Module TraceSemantics. Section trace_semantics.
 
-Context {G C : Type}.
+Context {G C Z : Type}.
 
-Variable sem : @EffectSem G C.
-Variable spec : ext_spec unit.
-Variable Espec : effect_spec.
+Variable z_init : Z.
+Variable sem : @CoopCoreSem G C.
+Variable spec : ext_spec Z.
 
-Inductive effstep : 
-  G -> 
-  (block -> BinNums.Z -> bool) -> 
-  (list Event.t*C) -> mem -> (list Event.t*C) -> mem -> Prop :=
-| trace_stepplus :
-  forall ge U tr c m c' m',
-  effstep_plus sem ge U c m c' m' -> 
-  effstep ge U (tr,c) m (tr,c') m'
-| trace_extstep : 
-  forall ge U tr c m c' m' ef sig args rv x,
+Definition yielded c :=
+  exists ef sig args, at_external sem c = Some (ef, sig, args) 
+  \/ exists rv, halted sem c = Some rv.
+
+Inductive step : G -> (Z*list Event.t*C) -> mem -> (Z*list Event.t*C) -> mem -> Prop :=
+| trace_step :
+  forall ge tr z c m c' m',
+  corestep_plus sem ge c m c' m' -> 
+  yielded c' -> 
+  step ge (z,tr,c) m (z,tr,c') m'
+| trace_extern : 
+  forall ge tr z c m z' c' m' ef sig args rv x,
   at_external sem c = Some (ef, sig, args) -> 
-  (forall b ofs, Mem.valid_block m b -> Espec ef args m b ofs=true -> U b ofs=true) -> 
-  Mem.unchanged_on (fun b ofs => U b ofs = false) m m' ->   
+  Mem.unchanged_on (fun b ofs => REACH m (getBlocks args) b=false) m m' ->   
   mem_forward m m' -> 
-  ext_spec_pre spec ef x (sig_args sig) args tt m -> 
-  ext_spec_post spec ef x (sig_res sig) rv tt m' -> 
-  after_external sem rv c = Some c' -> 
-  effstep ge U (tr,c) m (Event.mk m m' args rv :: tr,c') m'.
+  ext_spec_pre spec ef x (sig_args sig) args z m -> 
+  ext_spec_post spec ef x (sig_res sig) (Some rv) z' m' -> 
+  after_external sem (Some rv) c = Some c' -> 
+  step ge (z,tr,c) m (z',Event.mk m m' args (Some rv) :: tr,c') m'.
 
-Definition step ge c m c' m' := exists U, effstep ge U c m c' m'.
-
-Definition initial_core (ge : G) (v : val) (vs : list val) : option (list Event.t*C) := 
+Definition initial_core (ge : G) (v : val) (vs : list val) 
+  : option (Z*list Event.t*C) := 
   match initial_core sem ge v vs with 
-    | Some c => Some (nil, c)
+    | Some c => Some (z_init, nil, c)
     | None => None
   end.
 
-Definition halted (c : list Event.t*C) := halted sem (snd c).
+Definition halted (c : Z*list Event.t*C) := halted sem (snd c).
 
-Program Definition coresem : CoreSemantics G (list Event.t*C) mem :=
-  @Build_CoreSemantics G (list Event.t*C) mem 
+Program Definition coresem : CoreSemantics G (Z*list Event.t*C) mem :=
+  @Build_CoreSemantics G (Z*list Event.t*C) mem 
   initial_core
   (fun _ => None)
   (fun _ _ => None)
@@ -75,60 +75,25 @@ Program Definition coresem : CoreSemantics G (list Event.t*C) mem :=
   _ _ _ _.
 Next Obligation.
 destruct H.
-destruct H.
 destruct H as [n H].
 hnf in H.
 destruct H as [c2 [m2 [H1 H2]]].
-apply effax1 in H1.
-destruct H1 as [H1 ?].
 apply corestep_not_halted in H1.
 unfold halted.
 solve[auto].
 solve[destruct (at_external_halted_excl sem c1); try congruence; auto].
 Qed.
 
-Program Definition coopsem : CoopCoreSem G (list Event.t*C) :=
-  @Build_CoopCoreSem G (list Event.t*C) coresem _.
+Program Definition coopsem : CoopCoreSem G (Z*list Event.t*C) :=
+  @Build_CoopCoreSem G (Z*list Event.t*C) coresem _.
 Next Obligation.
-destruct CS.
-destruct H; auto.
+destruct CS; auto.
 destruct H as [n H].
 hnf in H.
 destruct H as [c2 [m2 [H1 H2]]].
-apply effstep_fwd in H1.
-apply effstepN_fwd in H2.
+apply corestep_fwd in H1.
+apply corestepN_fwd in H2.
 solve[eapply mem_forward_trans; eauto].
-Qed.
-
-Lemma effstep_sub_val : 
-  forall g U V c m c' m',
-  (forall b ofs, Mem.valid_block m b ->  U b ofs = true -> V b ofs = true) ->
-  effstep g U c m c' m' -> effstep g V c m c' m'.
-Proof.
-intros.
-destruct H0.
-constructor.
-solve[eapply effstep_plus_sub_val; eauto].
-econstructor; eauto.
-apply unch_on_validblock with (V := fun b ofs => U b ofs=false); auto.
-intros.
-case_eq (U b ofs); auto.
-intros A.
-generalize (H _ _ H7 A); congruence.
-Qed.
-
-Program Definition effsem : @EffectSem G (list Event.t*C) :=
-  @Build_EffectSem G (list Event.t*C) coopsem effstep _ _ effstep_sub_val.
-Next Obligation.
-destruct H.
-split; auto.
-exists U.
-constructor; auto.
-destruct H as [n H].
-solve[apply effstepN_unchanged in H; auto].
-constructor; auto.
-exists U.
-solve[eapply trace_extstep; eauto].
 Qed.
 
 End trace_semantics. End TraceSemantics.
